
## Variation 1
$$
<e, \epsilon> = 0 \text{ con P = 1}
$$
$$
\begin{align}
 & <m + <e,y>, <eA^{t}, s>  = m<eA^{t}, s> + <e,sA><eA^{t}, s>  \\
 & \text{se m = 0} \implies 0 + <<e,sA>eA^{t},s> + <eA^{t},<e,sA>s>
\end{align}
$$
Ad occhio direi che $P(<e, sA> = 1) = \frac{1}{2}$, in piu visto che se $<e,sA> = 0$ allora $m+<e,y> = 0$ nell'altro caso ho $<eA^{t},s>+<eA^{t},s>$ = 0
Se $m = 1$ allora mi rimane solo che $m<eA^t,s> = <eA^t,s>$ 


$$
<m + <e,y>, <eA^{t}, s> =m<eA^{t}, s> + <e,sA><eA^{t}, s> = m<eA^{t},s>
$$

Se $m = 1\implies$ decodifico 1 con $P=\frac{1}{2}$ 
Se $m = 0 \implies$ decodifico 0 con $P=1$
